ironfleet/src/IronfleetCommon/RSLClient.cs
@@ -12,21 +12,27 @@ namespace IronfleetCommon
     IPEndPoint[] serverEps;
     IPEndPoint myEp;
     IoScheduler scheduler;
-    SeqNumManager seqNumManager;
+    UInt64 nextSeqNum;
     int primaryServerIndex;
 
-    public RSLClient(IEnumerable<IPEndPoint> i_serverEps, IPEndPoint i_myEp, int seqNumReservationSize = 1000)
+    public RSLClient(IEnumerable<IPEndPoint> i_serverEps, IPEndPoint i_myEp)
     {
       serverEps = Enumerable.ToArray(i_serverEps);
       myEp = i_myEp;
       scheduler = new IoScheduler(myEp, true, false); // onlyClient = true, verbose = false
-      seqNumManager = new SeqNumManager(myEp.Port, seqNumReservationSize);
       primaryServerIndex = 0;
       Start();
     }
 
     private void Start()
     {
+      // Create a random 64-bit initial sequence number.
+
+      Random rng = new Random();
+      byte[] seqNumBytes = new byte[8];
+      rng.NextBytes(seqNumBytes);
+      nextSeqNum = IoEncoder.ExtractUInt64(seqNumBytes, 0);
+
       // Create connections to all endpoints, so that if any of them
       // sends a reply we can receive it.  Since we're in "only
       // client" mode, we aren't listening on any port so we have to
@@ -40,7 +46,7 @@ namespace IronfleetCommon
 
     public byte[] SubmitRequest (byte[] request, bool verbose = false, int timeBeforeServerSwitchMs = 1000)
     {
-      UInt64 seqNum = seqNumManager.Next;
+      UInt64 seqNum = nextSeqNum++;
       byte[] requestMessage;
       using (var memStream = new MemoryStream())
       {
@@ -51,13 +57,13 @@ namespace IronfleetCommon
         requestMessage = memStream.ToArray();
       }
 
+      scheduler.SendPacket(serverEps[primaryServerIndex], requestMessage);
+      if (verbose) {
+        Console.WriteLine("Sending a request with sequence number {0} to {1}", seqNum, serverEps[primaryServerIndex]);
+      }
+
       while (true)
       {
-        scheduler.SendPacket(serverEps[primaryServerIndex], requestMessage);
-        if (verbose) {
-          Console.WriteLine("Sending a request with sequence number {0} to {1}", seqNum, serverEps[primaryServerIndex]);
-        }
-
         bool ok, timedOut;
         IPEndPoint remote;
         byte[] replyBytes;
@@ -72,6 +78,7 @@ namespace IronfleetCommon
           if (verbose) {
             Console.WriteLine("#timeout; rotating to server {0}", primaryServerIndex);
           }
+          scheduler.SendPacket(serverEps[primaryServerIndex], requestMessage);
           continue;
         }
 
