ironfleet/src/Dafny/Distributed/Protocol/RSL/Executor.i.dfy
@@ -156,9 +156,9 @@ predicate LExecutorProcessRequest(s:LExecutor, inp:RslPacket, sent_packets:seq<R
   requires inp.msg.RslMessage_Request?
   requires inp.src in s.reply_cache
   requires s.reply_cache[inp.src].Reply?
-  requires inp.msg.seqno_req <= s.reply_cache[inp.src].seqno
+  requires inp.msg.seqno_req == s.reply_cache[inp.src].seqno
 {
-  if inp.msg.seqno_req == s.reply_cache[inp.src].seqno && LReplicaConstantsValid(s.constants) then
+  if LReplicaConstantsValid(s.constants) then
     var r := s.reply_cache[inp.src];
     sent_packets == [ LPacket(r.client, s.constants.all.config.replica_ids[s.constants.my_index], RslMessage_Reply(r.seqno, r.reply)) ]
   else
