ironfleet/src/Dafny/Distributed/Protocol/RSL/Replica.i.dfy
@@ -58,13 +58,23 @@ predicate LReplicaNextProcessRequest(s:LReplica, s':LReplica, received_packet:Rs
     && s' == s
   else if && received_packet.src in s.executor.reply_cache
           && s.executor.reply_cache[received_packet.src].Reply?
-          && received_packet.msg.seqno_req <= s.executor.reply_cache[received_packet.src].seqno then
+          && received_packet.msg.seqno_req == s.executor.reply_cache[received_packet.src].seqno then
+    // If the reply cache contains exactly the given sequence number, we must send
+    // the matching reply from our reply cache.
     && LExecutorProcessRequest(s.executor, received_packet, sent_packets)
     && s' == s
   else
-    && LProposerProcessRequest(s.proposer, s'.proposer, received_packet)
-    && sent_packets == []
-    && s' == s.(proposer := s'.proposer)
+    // This is either a fresh or an outdated request.  If it's fresh, we must propose it.
+    // If it's outdated, we can either ignore or propose it.
+    || (&& LProposerProcessRequest(s.proposer, s'.proposer, received_packet)
+       && sent_packets == []
+       && s' == s.(proposer := s'.proposer))
+
+    || (&& received_packet.src in s.executor.reply_cache
+       && s.executor.reply_cache[received_packet.src].Reply?
+       && received_packet.msg.seqno_req < s.executor.reply_cache[received_packet.src].seqno
+       && sent_packets == []
+       && s' == s)
 }
 
 predicate LReplicaNextProcess1a(s:LReplica, s':LReplica, received_packet:RslPacket, sent_packets:seq<RslPacket>)
